several edits on mutual cases

coq/Main.v
@@ -28,6 +28,14 @@ Inductive htype :=
 | HArr (A B : htype)
 | Hole (e : term).
 
+Fixpoint rename_htype (A : htype) Γ : htype :=
+  match A with
+  | HInt => HInt
+  | HTop => HTop
+  | HArr A B => HArr (rename_htype A Γ) (rename_htype B Γ)
+  | Hole e => Hole (e.[ren Γ])
+  end.
+
 Fixpoint type_is_htype (A : type) : htype :=
   match A with
   | Int => HInt
@@ -40,20 +48,20 @@ Coercion type_is_htype : type >-> htype.
 Inductive ty (Γ : var -> type) : htype -> term -> type -> Prop :=
 | Ty_Lit  A n :
   sub Γ Int A ->
-  ty Γ A (Lit n) Int
+  ty Γ A (Lit n) Int     
 | Ty_Var A B x :
   Γ x = B -> sub Γ B A ->
-  ty Γ A (Var x) B
+  ty Γ A (Var x) B     
 | Ty_App e1 e2 A C D :
   ty Γ (HArr (Hole e2) A) e1 (Arr C D) ->
-  ty Γ A (App e1 e2) D
+  ty Γ A (App e1 e2) D     
 | Ty_Ann A (B : type) C e :
   ty Γ B e C -> sub Γ B A ->
-  ty Γ A (Ann e B) B
+  ty Γ A (Ann e B) B     
 | Ty_Lam1 e1 e A B B':
   ty Γ Top e1 A ->
   ty (A .: Γ) B' e B ->
-  ty Γ (HArr (Hole e1) B') (Lam e) (Arr A B)
+  ty Γ (HArr (Hole e1) B') (Lam e) (Arr A B)     
 | Ty_Lam2 e A B' C :
   ty (A .: Γ) B' e C ->
   ty Γ (HArr A B') (Lam e) (Arr A C)
@@ -63,6 +71,8 @@ with sub (Γ : var -> type) : htype -> htype -> Prop :=
 | S_Arr A B C D : sub Γ C A -> sub Γ B D -> sub Γ (HArr A B) (HArr C D)
 | S_Hole A A' e : ty Γ A e A' -> sub Γ (Hole e) A.
 
+Scheme ty_mut := Induction for ty Sort Prop with sub_mut := Induction for sub Sort Prop.
+
 Notation "A → B" := (Arr A B) (at level 20).
 Notation "A *→ B" := (HArr A B) (at level 20).
 Notation "⟦ e ⟧" := (Hole e) (at level 20).
@@ -71,25 +81,51 @@ Notation "G ⊢ A ⇒ e ⇒ B" := (ty G A e B) (at level 50).
 Notation "G ⊢ A <: B" := (sub G A B) (at level 50).
 
 (** Weakening Lemma *)
+Check sub_ind.
+Check sub_mut.
 
-Lemma sub_ren Γ A B:
+Lemma rename_type_eq : forall (t : type) ξ, rename_htype t ξ = t.
+Proof.
+  intros. induction t; eauto.
+  simpl in *. rewrite IHt1. rewrite IHt2.
+  auto.
+Qed.
+
+Lemma sub_ren' Γ A B:
   sub Γ A B -> forall Δ ξ, Γ = ξ >>> Δ -> sub Δ A B.
 Proof.
-  intros. subst. dependent induction H; eauto.
-  - econstructor.
-  - econstructor.
-  - econstructor; eauto.
+  intros. induction H.
   - econstructor.
 Admitted.
+  
 
+Lemma sub_ren :
+  forall Γ A B, sub Γ A B -> forall Δ ξ, Γ = ξ >>> Δ -> sub Δ (rename_htype A ξ) (rename_htype B ξ).
+Proof.
+  
+  Check sub_mut.
+  intros Γ A B H.
+  pattern Γ, A, B, H.
+  eapply sub_mut with
+    (
+      P := fun Γ A e B h => forall Δ ξ, Γ = ξ >>> Δ -> ty Δ (rename_htype A ξ) e.[ren ξ] B
+    )
+  ; intros; eauto.
+  - simpl in *. eapply Ty_Lit; eauto.
+  - subst. simpl in *. econstructor; eauto.
+    specialize (H0 Δ ξ (eq_refl _)).
+    rewrite (rename_type_eq _ _) in H0.
+    auto.
+  - admit.
+  - admit.
+  - admit.
+  - 
+Admitted.
 
 Lemma ty_ren Γ e A B:
   ty Γ B e A -> forall Δ ξ, Γ = ξ >>> Δ -> ty Δ B e.[ren ξ] A.
 Proof.
-  induction 1; intros.
-  - simpl. apply Ty_Lit; eauto.
-    eapply sub_ren; eauto.
-Admitted.          
+Admitted.
   
 Lemma ty_sub : forall A B e G,
     ty G A e B ->
